cedar-lean/Cedar/Thm/Validation/WellTyped/Record.lean
@@ -16,6 +16,7 @@
 
 import Cedar.Validation.TypedExpr
 import Cedar.Thm.Validation.WellTyped.Definition
+import Cedar.Thm.Validation.Typechecker.Record
 import Cedar.Thm
 import Cedar.Spec
 
@@ -25,51 +26,95 @@ open Cedar.Validation
 open Cedar.Thm
 open Cedar.Spec
 
-theorem well_typed_is_sound_set
+theorem attr_value_has_attrType
+{env : Environment}
+{request : Request}
+{entities : Entities}
+{m : List (Attr × TypedExpr)}
+{r : List (Attr × Value)}
+{rty : List (Attr × QualifiedType)}
+(h₁ : RequestAndEntitiesMatchEnvironment env request entities)
+(h₂ : ∀ (k : Attr) (v : TypedExpr), (k, v) ∈ m → WellTypedIsSound v)
+(h₃ : ∀ (k : Attr) (v : TypedExpr), (k, v) ∈ m → TypedExpr.WellTyped env v)
+(h₄ : List.Forall₂ (λ x y => x.fst = y.fst ∧ x.snd.typeOf = Qualified.getType y.snd) m rty)
+(h₅ : List.Forall₂ (λ x y => Prod.mk x.fst <$> evaluate x.snd.toExpr request entities = Except.ok y) m r) :
+List.Forall₂ (λ x y => x.fst = y.fst ∧ InstanceOfType x.snd (Qualified.getType y.snd)) r rty
+:= by
+  cases h₄ <;> cases h₅
+  case nil.nil => simp only [List.Forall₂.nil]
+  case cons.cons at₁ aq₁ at₂ aq₂ hᵢ₁ hᵢ₂ av lv hᵢ₃ hᵢ₄ =>
+    have h : (at₁.fst, at₁.snd) ∈ at₁ :: at₂ := by
+        simp only [List.mem_cons, true_or]
+    have h₂₁ : WellTypedIsSound at₁.snd := by
+      exact h₂ at₁.fst at₁.snd h
+    have h' : ∀ (k : Attr) (v : TypedExpr), (k, v) ∈ at₂ → (k, v) ∈ at₁ :: at₂ := by
+      intro k v
+      simp [List.mem_cons_of_mem]
+      intro a
+      right
+      exact a
+    have h₂₂ : ∀ (k : Attr) (v : TypedExpr), (k, v) ∈ at₂ → WellTypedIsSound v := by
+      intro k v h
+      exact h₂ k v (h' k v h)
+    have h₃₁ : TypedExpr.WellTyped env at₁.snd := by
+      exact h₃ at₁.fst at₁.snd h
+    have h₃₂ : ∀ (k : Attr) (v : TypedExpr), (k, v) ∈ at₂ → TypedExpr.WellTyped env v := by
+      intro k v h
+      exact h₃ k v (h' k v h)
+    generalize hᵢ₃' : evaluate at₁.snd.toExpr request entities = res
+    cases res
+    case error => simp only [hᵢ₃', Except.map_error, reduceCtorEq] at hᵢ₃
+    case ok v =>
+      simp only [hᵢ₃', Except.map_ok, Except.ok.injEq] at hᵢ₃
+      simp only [WellTypedIsSound] at h₂₁
+      replace h₂₁ := h₂₁ h₁ h₃₁ hᵢ₃'
+      obtain ⟨hᵢ₁₁, hᵢ₁₂⟩ := hᵢ₁
+      have hᵢ := attr_value_has_attrType h₁ h₂₂ h₃₂ hᵢ₂ hᵢ₄
+      have h' : av = (av.fst, av.snd) := by rfl
+      rw [h'] at hᵢ₃
+      simp only [Prod.mk.injEq] at hᵢ₃
+      obtain ⟨hᵢ₃₁, hᵢ₃₂⟩ := hᵢ₃
+      have h : av.fst = aq₁.fst ∧ InstanceOfType av.snd (Qualified.getType aq₁.snd) := by
+        rw [←hᵢ₁₁]
+        simp only [hᵢ₃₁, true_and]
+        simp only [hᵢ₃₂, hᵢ₁₂] at h₂₁
+        exact h₂₁
+      exact List.Forall₂.cons h hᵢ
+
+
+theorem well_typed_is_sound_record
 {v : Value}
 {env : Environment}
 {request : Request}
 {entities : Entities}
-{rty : RecordType}
 {m : List (Attr × TypedExpr)}
+{rty : List (Attr × QualifiedType)}
 (h₁ : RequestAndEntitiesMatchEnvironment env request entities)
 (h₂ : ∀ (k : Attr) (v : TypedExpr), (k, v) ∈ m → WellTypedIsSound v)
 (h₃ : ∀ (k : Attr) (v : TypedExpr), (k, v) ∈ m → TypedExpr.WellTyped env v)
-(h₄ : rty =
-  Data.Map.make
-    (List.map
-      (λ x =>
-        match x with
-        | (a, ty) => (a, Qualified.required ty.typeOf))
-      m))
+(h₄ : List.Forall₂ (λ x y => x.fst = y.fst ∧ x.snd.typeOf = Qualified.getType y.snd) m rty)
 (h₅ : (do
   let avs ←
-  (List.map (fun x => (x.1.fst, x.1.snd.toExpr)) m.attach₂).mapM₂ fun x =>
+  (List.map (λ x => (x.1.fst, x.1.snd.toExpr)) m.attach₂).mapM₂ λ x =>
   bindAttr x.1.fst (evaluate x.1.snd request entities)
   Except.ok (Value.record (Data.Map.make avs))) = Except.ok v) :
-InstanceOfType v (TypedExpr.record m (CedarType.record rty)).typeOf
+InstanceOfType v (TypedExpr.record m (CedarType.record (Data.Map.make rty))).typeOf
 := by
   simp only [do_ok] at h₅
   obtain ⟨r, h₅₁, h₅₂⟩ := h₅
-  simp only [← h₅₂, TypedExpr.typeOf]
+  subst h₅₂
   rw [List.map_attach₂ (fun x : Attr × TypedExpr => (x.fst, x.snd.toExpr))] at h₅₁
   simp only [List.mapM₂, List.attach₂] at h₅₁
   simp only [List.mapM_pmap_subtype
       (fun (x : Attr × Expr) => bindAttr x.fst (evaluate x.snd request entities))] at h₅₁
   simp only [bindAttr, bind_pure_comp, List.mapM_map, List.mapM_ok_iff_forall₂] at h₅₁
-
-
-  have h₆ : ∀ (k : Attr), (Data.Map.make r).contains k → rty.contains k := by
-    sorry
-
-  have h₇ : ∀ (k : Attr) (v : Value) (qty : QualifiedType),
-    (Data.Map.make r).find? k = some v → rty.find? k = some qty → InstanceOfType v qty.getType := by
-    sorry
-
-  have h₈ : ∀ (k : Attr) (qty : QualifiedType), rty.find? k = some qty →
-    qty.isRequired → (Data.Map.make r).contains k := by
-    sorry
-
-  exact InstanceOfType.instance_of_record (Data.Map.make r) rty h₆ h₇ h₈
+  have h₅ : List.Forall₂ AttrValueHasAttrType r rty := by
+    exact attr_value_has_attrType h₁ h₂ h₃ h₄ h₅₁
+  simp [TypedExpr.typeOf]
+  apply mk_vals_instance_of_mk_types
+  let p := fun (v : Value) (qty : QualifiedType) => InstanceOfType v qty.getType
+  have h₆ := List.canonicalize_preserves_forallᵥ p r rty
+  simp only [List.Forallᵥ] at h₆
+  exact h₆ h₅
 
 end Cedar.Thm
